spec/abstract/Tcb_A.thy
@@ -262,7 +262,7 @@ definition
      cur \<leftarrow> gets cur_thread;
      tcb_sched_action tcb_sched_dequeue tptr;
      thread_set_domain tptr new_dom;
-     sched \<leftarrow> is_schedulable tptr;
+     sched \<leftarrow> gets (schedulable tptr);
      when sched $ tcb_sched_action tcb_sched_enqueue tptr; \<comment> \<open>schedulable and dequeued\<close>
      when (tptr = cur) $ reschedule_required
    od"
